Semantic/CC/Syntax/Exp.lean
@@ -40,6 +40,8 @@ def Exp.rename : Exp s1 -> Rename s1 s2 -> Exp s2
 | .unit, _ => .unit
 | .btrue, _ => .btrue
 | .bfalse, _ => .bfalse
+| .read x, f => .read (x.rename f)
+| .write x y, f => .write (x.rename f) (y.rename f)
 | .cond x e2 e3, f => .cond (x.rename f) (e2.rename f) (e3.rename f)
 
 /-- An expression is a value if it is an abstraction, pack, or unit. -/
@@ -136,6 +138,8 @@ inductive Exp.IsClosed : Exp s -> Prop where
 | unit : Exp.IsClosed .unit
 | btrue : Exp.IsClosed .btrue
 | bfalse : Exp.IsClosed .bfalse
+| read : Var.IsClosed x -> Exp.IsClosed (.read x)
+| write : Var.IsClosed x -> Var.IsClosed y -> Exp.IsClosed (.write x y)
 | cond : Var.IsClosed x -> Exp.IsClosed e2 -> Exp.IsClosed e3 -> Exp.IsClosed (.cond x e2 e3)
 
 end CC
